src/Narcissus/Automation/SynthesizeDecoder.v
@@ -94,42 +94,49 @@ Ltac apply_base_rule :=
   (* Word *)
   | H : cache_inv_Property _ _
     |- context [CorrectDecoder _ _ _ _ format_word _ _ _] =>
-    intros; eapply (Word_decode_correct H); throw "Could not synthesize decoder for word."%string
+    intros;
+    first [ solve [eapply (Word_decode_correct H)]
+          | throw "Could not synthesize decoder for word."%string ]
 
   (* Natural Numbers *)
   | H : cache_inv_Property _ _
     |- context [CorrectDecoder _ _ _ _ (format_nat _) _ _ _] =>
-    intros; revert H; eapply Nat_decode_correct; throw "Could not synthesize decoder for nat."%string
+    intros; revert H;
+    first [ solve [eapply Nat_decode_correct]
+          | throw "Could not synthesize decoder for nat."%string ]
 
   (* Booleans *)
   | H : cache_inv_Property _ _
     |- context [CorrectDecoder _ _ _ _ (format_bool) _ _ _] =>
-    intros; revert H; eapply bool_decode_correct; throw "Could not synthesize decoder for boolean."%string
+    first [ solve [intros; revert H; eapply bool_decode_correct]
+          | throw "Could not synthesize decoder for boolean."%string ]
 
   (* Strings *)
   | H : cache_inv_Property _ _
   |- context[CorrectDecoder _ _ _ _ StringOpt.format_string _ _ _ ] =>
-    eapply (StringOpt.String_decode_correct _ H); throw "Could not synthesize decoder for string."%string
+    first [ solve [eapply (StringOpt.String_decode_correct _ H)]
+          | throw "Could not synthesize decoder for string."%string ]
 
   (* Enumerated Types *)
   | H : cache_inv_Property _ _
     |- context [CorrectDecoder _  _ _ _ (format_enum ?tb) _ _ _] =>
-    intros;
-    eapply (fun NoDup => @Enum_decode_correct _ _ _ _ _ _ _ tb NoDup _ H);
-    solve_side_condition;
-    throw "Could not synthesize decoder for enum."%string
+    intros; eapply (fun NoDup => @Enum_decode_correct _ _ _ _ _ _ _ tb NoDup _ H);
+    first [ solve [solve_side_condition]
+          | throw "Could not synthesize decoder for enum."%string ]
 
   (* Unused words *)
   | |- context [CorrectDecoder _  _ _ _ (format_unused_word _) _ _ _] =>
-    intros; eapply unused_word_decode_correct; eauto;
-    throw "Could not synthesize decoder for unused word."%string
+    intros; eapply unused_word_decode_correct;
+    first [ solve[eauto]
+          | throw "Could not synthesize decoder for unused word."%string ]
 
   (* ByteBuffers *)
   | H : cache_inv_Property ?mnd _
     |- CorrectDecoder _ _ _ _ format_bytebuffer _ _ _ =>
     intros; eapply @ByteBuffer_decode_correct;
-    first [exact H | solve [intros; intuition eauto] ];
-    throw "Could not synthesize decoder for byte buffer."%string
+    first [ exact H
+          | solve [intros; intuition eauto]
+          | throw "Could not synthesize decoder for byte buffer."%string ]
 
   (* Hook for new base rules. *)
   | |- _ => apply_new_base_rule
