src/Narcissus/Examples/Errors/FormatList/ActuallyByteAligned.v
@@ -11,5 +11,8 @@ Definition invariant (m : msg) :=
 Definition dec : Maybe (CorrectAlignedDecoderFor invariant format).
 Proof.
   maybe_synthesize_aligned_decoder.
-  Show Proof.
 Defined.
+
+Let dec' := Eval simpl in extractDecoder dec.
+Print dec'.
+Print Assumptions dec'.
