src/Narcissus/Examples/Errors/FormatList/NotByteAligned.v
@@ -10,5 +10,8 @@ Definition invariant (m : msg) := length (m.(data)) < pow2 8.
 Definition dec : Maybe (CorrectAlignedDecoderFor invariant format).
 Proof.
   maybe_synthesize_aligned_decoder.
-  Show Proof.
 Defined.
+
+Let dec' := Eval simpl in extractDecoder dec.
+Print dec'.
+Print Assumptions dec'.
