src/Narcissus/Examples/Errors/FormatString/StringConst.v
@@ -11,8 +11,11 @@ Definition invariant (_ : msg) := True.
 Definition dec : Maybe (CorrectAlignedDecoderFor invariant format).
 Proof.
   maybe_synthesize_aligned_decoder.
-  Show Proof.
   (* More of a limitation than error: need to fix [solve_side_condition], add
   a decides instance, disallow simplifying the decoder function, and add a
   [DecodeMEquivAlignedDecodeM] instance. *)
 Defined.
+
+Let dec' := Eval simpl in extractDecoder dec.
+Print dec'.
+Print Assumptions dec'.
